Moved generalized setup2/2_i definitions and wow-lemmas to call_lemmas. These now support non-empty type lists. Previous lemmas are retained (with names ending in ...nil), and are proven as specializtions of the full lemmas. Adapted tactics in forward to (for now) call on the ...-nil lemmas

floyd/call_lemmas.v
@@ -917,6 +917,47 @@ subst ty.
 auto.
 Qed.
 
+Definition call_setup2
+  (cs: compspecs) Qtemp Qvar GV a Delta P Q R R'
+   fs argsig retty cc ts (A: rmaps.TypeTree)  Pre Post NEPre NEPost
+  (bl: list expr) (vl : list val)
+  (Qactuals : PTree.t _)
+  (witness: functors.MixVariantFunctor._functor (rmaps.dependent_type_functor_rec ts A) mpred)
+  (Frame: list mpred)
+  (Ppre: list Prop) (Qpre : list localdef) (Rpre: list mpred)
+  (Qpre_temp : PTree.t _) GV' :=
+ call_setup1 cs Qtemp Qvar GV a Delta P Q (*R*)R' fs argsig retty cc A Pre Post NEPre NEPost bl vl Qactuals /\
+(*moved here from setup1*)  PROPx P (LOCALx Q (SEPx R')) |-- |> PROPx P (LOCALx Q (SEPx R)) /\ 
+  Pre ts witness = PROPx Ppre (LOCALx Qpre (SEPx Rpre)) /\
+  local2ptree Qpre = (Qpre_temp, PTree.empty _, nil, GV') /\
+  ENTAIL Delta, PROPx P (LOCALx Q (SEPx R')) (*WAS R*)
+           |-- !! Forall (check_one_temp_spec Qactuals) (PTree.elements Qpre_temp) /\
+  check_gvars_spec GV GV' /\
+  fold_right_sepcon R |-- fold_right_sepcon Rpre * fold_right_sepcon Frame.
+
+Lemma call_setup2_i:
+ forall  (cs: compspecs) Qtemp Qvar GV a Delta P Q R R'
+   fs argsig retty cc ts (A: rmaps.TypeTree) Pre Post NEPre NEPost
+  (bl: list expr) (vl : list val)
+  (Qactuals : PTree.t _)
+  (SETUP1: call_setup1 cs Qtemp Qvar GV a Delta P Q (*R*)R' fs argsig retty cc A Pre Post NEPre NEPost bl vl Qactuals)
+  (witness': functors.MixVariantFunctor._functor (rmaps.dependent_type_functor_rec ts A) mpred)
+  (Frame: list mpred)
+  (Ppre: list Prop) (Qpre : list localdef) (Rpre: list mpred)
+  (Qpre_temp : PTree.t _) GV',
+  Pre ts witness' = PROPx Ppre (LOCALx Qpre (SEPx Rpre)) ->
+  local2ptree Qpre = (Qpre_temp, PTree.empty _, nil, GV') ->
+  ENTAIL Delta, PROPx P (LOCALx Q (SEPx R')) (*WAS R*)
+           |-- !! Forall (check_one_temp_spec Qactuals) (PTree.elements Qpre_temp) ->
+(*moved here from setup1*)  PROPx P (LOCALx Q (SEPx R')) |-- |> PROPx P (LOCALx Q (SEPx R)) ->
+  check_gvars_spec GV GV' ->
+  fold_right_sepcon R |-- fold_right_sepcon Rpre * fold_right_sepcon Frame ->
+  call_setup2 cs Qtemp Qvar GV a Delta P Q R R' fs argsig retty cc ts A Pre Post NEPre NEPost bl vl Qactuals
+      witness' Frame Ppre Qpre Rpre Qpre_temp GV'.
+Proof.
+ intros. split. auto. repeat split; auto.
+Qed.
+(*
 Definition OLDcall_setup2 
   (cs: compspecs) Qtemp Qvar GV a Delta P Q R R'
    fs argsig retty cc (A: rmaps.TypeTree)  Pre Post NEPre NEPost
@@ -933,8 +974,9 @@ Definition OLDcall_setup2
            |-- !! Forall (check_one_temp_spec Qactuals) (PTree.elements Qpre_temp) /\
   check_gvars_spec GV GV' /\
   fold_right_sepcon R |-- fold_right_sepcon Rpre * fold_right_sepcon Frame.
+ *)
 
-Definition call_setup2 
+Definition call_setup2_nil 
   (cs: compspecs) Qtemp Qvar GV a Delta P Q R R'
    fs argsig retty cc (A: rmaps.TypeTree)  Pre Post NEPre NEPost
   (bl: list expr) (vl : list val)
@@ -952,7 +994,24 @@ Definition call_setup2
   check_gvars_spec GV GV' /\
   fold_right_sepcon R |-- fold_right_sepcon Rpre * fold_right_sepcon Frame.
 
-Lemma OLDcall_setup2_i:
+Lemma call_setup2_nil_equiv:
+  forall (cs: compspecs) Qtemp Qvar GV a Delta P Q R R'
+   fs argsig retty cc (A: rmaps.TypeTree)  Pre Post NEPre NEPost
+  (bl: list expr) (vl : list val)
+  (Qactuals : PTree.t _)
+  (witness: functors.MixVariantFunctor._functor (rmaps.dependent_type_functor_rec nil A) mpred)
+  (Frame: list mpred)
+  (Ppre: list Prop) (Qpre : list localdef) (Rpre: list mpred)
+  (Qpre_temp : PTree.t _) GV',
+    call_setup2_nil cs Qtemp Qvar GV a Delta P Q R R'
+                    fs argsig retty cc A Pre Post NEPre NEPost bl vl
+                    Qactuals witness Frame Ppre Qpre Rpre Qpre_temp GV' =
+    call_setup2 cs Qtemp Qvar GV a Delta P Q R R'
+                    fs argsig retty cc nil A Pre Post NEPre NEPost bl vl
+                    Qactuals witness Frame Ppre Qpre Rpre Qpre_temp GV'.
+reflexivity. Qed.
+   
+(*Lemma OLDcall_setup2_i:
  forall  (cs: compspecs) Qtemp Qvar GV a Delta P Q R R'
    fs argsig retty cc (A: rmaps.TypeTree)  Pre Post NEPre NEPost
   (bl: list expr) (vl : list val)
@@ -972,8 +1031,9 @@ Lemma OLDcall_setup2_i:
       witness' Frame Ppre Qpre Rpre Qpre_temp GV'.
 Proof.
  intros. split. auto. repeat split; auto.
-Qed.
-Lemma call_setup2_i:
+Qed.*)
+
+Lemma call_setup2_i_nil:
  forall  (cs: compspecs) Qtemp Qvar GV a Delta P Q R R'
    fs argsig retty cc (A: rmaps.TypeTree)  Pre Post NEPre NEPost
   (bl: list expr) (vl : list val)
@@ -990,11 +1050,12 @@ Lemma call_setup2_i:
 (*moved here from setup1*)  PROPx P (LOCALx Q (SEPx R')) |-- |> PROPx P (LOCALx Q (SEPx R)) ->
   check_gvars_spec GV GV' ->
   fold_right_sepcon R |-- fold_right_sepcon Rpre * fold_right_sepcon Frame ->
-  call_setup2 cs Qtemp Qvar GV a Delta P Q R R' fs argsig retty cc A Pre Post NEPre NEPost bl vl Qactuals
+  call_setup2_nil cs Qtemp Qvar GV a Delta P Q R R' fs argsig retty cc A Pre Post NEPre NEPost bl vl Qactuals
       witness' Frame Ppre Qpre Rpre Qpre_temp GV'.
 Proof.
  intros. split. auto. repeat split; auto.
 Qed.
+
 
 Lemma OLDactual_value_not_Vundef:
  forall (cs: compspecs) (Qtemp: PTree.t val) (Qvar: PTree.t (type * val))
@@ -1353,15 +1414,16 @@ rewrite later_andp; apply andp_right.
   eapply check_specs_lemma; try eassumption.
 Qed.
  *)
+
 Lemma semax_call_aux55:
  forall (cs: compspecs) (Qtemp: PTree.t val) (Qvar: PTree.t (type * val)) GV (a: expr)
-     Delta P Q R R' fs argsig retty (*cc*) 
-    (A : rmaps.TypeTree)
+     Delta P Q R R' fs argsig retty (*cc ts A Pre Post NEPre NEPost  *)
+    ts (A : rmaps.TypeTree)
          (Pre
           Post : forall ts : list Type,
               functors.MixVariantFunctor._functor
                 (rmaps.dependent_type_functor_rec
-                   ts (AssertTT A)) mpred) (* NEPre NEPost *) 
+                   ts (AssertTT A)) mpred) 
     witness Frame bl Ppre Qpre Rpre Qactuals Qpre_temp GV' vl
  (PTREE : local2ptree Q = (Qtemp, Qvar, nil, GV))
 (* (TC0 : ENTAIL Delta, PROPx P (LOCALx Q (SEPx R)) |-- tc_expr Delta a)
@@ -1370,10 +1432,10 @@ Lemma semax_call_aux55:
  (MSUBST : force_list (map (msubst_eval_expr Delta Qtemp Qvar GV)
               (explicit_cast_exprlist (argtypes argsig) bl)) = Some vl)
  (PTREE'' : pTree_from_elements (combine (var_names argsig) vl) = Qactuals)
- (PRE1 : Pre nil witness = PROPx Ppre (LOCALx Qpre (SEPx Rpre)))
+ (PRE1 : Pre ts witness = PROPx Ppre (LOCALx Qpre (SEPx Rpre)))
  (PTREE' : local2ptree Qpre = (Qpre_temp, PTree.empty _, nil, GV')) 
  (CHECKTEMP : Forall (check_one_temp_spec Qactuals) (PTree.elements Qpre_temp))
- (CHECKG: check_gvars_spec GV GV')
+ (CHECKG: check_gvars_spec GV GV' )
 (*moved here from setup1*)  (HR': PROPx P (LOCALx Q (SEPx R')) |-- |> PROPx P (LOCALx Q (SEPx R)))
  (FRAME : fold_right_sepcon R
            |-- fold_right_sepcon Rpre * fold_right_sepcon Frame)
@@ -1381,15 +1443,15 @@ Lemma semax_call_aux55:
  (LEN : length (argtypes argsig) = length bl),
 ENTAIL Delta, tc_expr Delta a && tc_exprlist Delta (argtypes argsig) bl &&
 (EX v : val,
- lift0 (func_ptr fs (* (mk_funspec (argsig, retty) cc A Pre Post NEPre NEPost) *) v) &&
+ lift0 (func_ptr fs v) &&
  local (` (eq v) (eval_expr a))) && PROPx P (LOCALx Q (SEPx R'))
 |-- (*|>*) (tc_expr Delta a && tc_exprlist Delta (argtypes argsig) bl) &&
-    (|> @liftx (Tarrow environ (LiftEnviron mpred)) (Pre nil witness)
+    (|> @liftx (Tarrow environ (LiftEnviron mpred)) (Pre ts witness)
        (make_args' (argsig, retty) (eval_exprlist (argtypes argsig) bl)) *
-     ` (func_ptr' fs (* (mk_funspec (argsig, retty) cc A Pre Post NEPre NEPost) *) )
+     ` (func_ptr' fs)
        (eval_expr a) * |>PROPx P (LOCALx Q (SEPx Frame))).
- Proof.
-   intros.
+Proof.
+intros.
 pose proof actual_value_not_Vundef _ _ _ _ P _ R _ _ _ _ PTREE (*TC1*) MSUBST as VUNDEF.
 rewrite <- ! andp_assoc.
 rewrite (andp_comm _ (EX v : val, lift0 (func_ptr fs v) && local ((` (eq v)) (eval_expr a)))%assert).
@@ -1486,6 +1548,139 @@ rewrite later_andp; apply andp_right.
   eapply check_specs_lemma; try eassumption.
 Qed.
 
+Lemma semax_call_aux55_nil:
+ forall (cs: compspecs) (Qtemp: PTree.t val) (Qvar: PTree.t (type * val)) GV (a: expr)
+     Delta P Q R R' fs argsig retty (*cc*) 
+    (A : rmaps.TypeTree)
+         (Pre
+          Post : forall ts : list Type,
+              functors.MixVariantFunctor._functor
+                (rmaps.dependent_type_functor_rec
+                   ts (AssertTT A)) mpred) (* NEPre NEPost *) 
+    witness Frame bl Ppre Qpre Rpre Qactuals Qpre_temp GV' vl
+ (PTREE : local2ptree Q = (Qtemp, Qvar, nil, GV))
+(* (TC0 : ENTAIL Delta, PROPx P (LOCALx Q (SEPx R)) |-- tc_expr Delta a)
+ (TC1 : ENTAIL Delta, PROPx P (LOCALx Q (SEPx R))
+             |-- tc_exprlist Delta (argtypes argsig) bl)*)
+ (MSUBST : force_list (map (msubst_eval_expr Delta Qtemp Qvar GV)
+              (explicit_cast_exprlist (argtypes argsig) bl)) = Some vl)
+ (PTREE'' : pTree_from_elements (combine (var_names argsig) vl) = Qactuals)
+ (PRE1 : Pre nil witness = PROPx Ppre (LOCALx Qpre (SEPx Rpre)))
+ (PTREE' : local2ptree Qpre = (Qpre_temp, PTree.empty _, nil, GV')) 
+ (CHECKTEMP : Forall (check_one_temp_spec Qactuals) (PTree.elements Qpre_temp))
+ (CHECKG: check_gvars_spec GV GV')
+(*moved here from setup1*)  (HR': PROPx P (LOCALx Q (SEPx R')) |-- |> PROPx P (LOCALx Q (SEPx R)))
+ (FRAME : fold_right_sepcon R
+           |-- fold_right_sepcon Rpre * fold_right_sepcon Frame)
+ (PPRE : fold_right_and True Ppre)
+ (LEN : length (argtypes argsig) = length bl),
+ENTAIL Delta, tc_expr Delta a && tc_exprlist Delta (argtypes argsig) bl &&
+(EX v : val,
+ lift0 (func_ptr fs (* (mk_funspec (argsig, retty) cc A Pre Post NEPre NEPost) *) v) &&
+ local (` (eq v) (eval_expr a))) && PROPx P (LOCALx Q (SEPx R'))
+|-- (*|>*) (tc_expr Delta a && tc_exprlist Delta (argtypes argsig) bl) &&
+    (|> @liftx (Tarrow environ (LiftEnviron mpred)) (Pre nil witness)
+       (make_args' (argsig, retty) (eval_exprlist (argtypes argsig) bl)) *
+     ` (func_ptr' fs (* (mk_funspec (argsig, retty) cc A Pre Post NEPre NEPost) *) )
+       (eval_expr a) * |>PROPx P (LOCALx Q (SEPx Frame))).
+ Proof. intros. eapply semax_call_aux55 with (ts:=nil); eassumption. Qed.
+(*original proof:
+pose proof actual_value_not_Vundef _ _ _ _ P _ R _ _ _ _ PTREE (*TC1*) MSUBST as VUNDEF.
+rewrite <- ! andp_assoc.
+rewrite (andp_comm _ (EX v : val, lift0 (func_ptr fs v) && local ((` (eq v)) (eval_expr a)))%assert).
+rewrite ! andp_assoc.
+rewrite !exp_andp1. Intros v.
+repeat apply andp_right; auto; try solve [ solve_andp].
+rewrite andp_comm. rewrite andp_assoc. (*
+{ do 2 apply andp_left2. eapply derives_trans(*, later_derives*), TC0.
+  rewrite later_andp; apply andp_derives; [apply now_later|].
+  apply andp_left2. derives_refl. }
+{ eapply derives_trans, later_derives, TC1.
+  rewrite later_andp; apply andp_derives; [apply now_later|].
+  apply andp_left2, derives_refl. }*)
+rewrite PRE1.
+match goal with |- _ |-- ?A * ?B * ?C => pull_right B end.
+rewrite sepcon_comm.
+rewrite func_ptr'_func_ptr_lifted.
+apply ENTAIL_trans with
+ (`(func_ptr fs) (eval_expr a) && (tc_exprlist Delta (argtypes argsig) bl &&
+   |>PROPx P (LOCALx Q (SEPx R)))).
+{ 
+  apply andp_left2. rewrite <- andp_assoc.
+  apply andp_right. (*[| solve_andp].*)
+  + rewrite ! andp_assoc.  do 3 apply andp_left2.
+    intro rho; unfold_lift; unfold local, lift0, lift1; simpl. normalize.
+  + apply andp_right. solve_andp. do 2 apply andp_left1. do 2 apply andp_left2. trivial.  }
+  
+apply andp_right.
+{ apply andp_left2; apply andp_left1; auto. }
+forget (tc_exprlist Delta (argtypes argsig) bl) as TCEXPRLIST.
+eapply derives_trans;[ apply andp_derives; [apply derives_refl | apply andp_left2; apply derives_refl] |].
+subst Qactuals.
+clear - PTREE LEN PTREE' MSUBST FRAME PPRE CHECKTEMP CHECKG VUNDEF.
+rewrite <- later_sepcon.
+ progress (autorewrite with norm1 norm2).
+rewrite PROP_combine.
+rewrite (andp_comm (local (fold_right _ _ _))).
+rewrite later_andp; apply andp_right.
++
+  apply andp_left2. apply andp_left2. apply later_derives.
+(*  apply derives_trans with (|> (TCEXPRLIST && PROPx P (LOCALx Q (SEPx R)))).
+  { rewrite later_andp. apply andp_derives; [ apply now_later | trivial].  }
+  apply later_derives. apply andp_left2.*)
+  apply andp_right.
+  apply andp_left1.
+  rewrite fold_right_and_app_low.
+  apply prop_derives; intros; split; auto.
+  clear - PPRE.
+  revert PPRE; induction Ppre; simpl; intuition.
+  apply andp_left2.
+  apply andp_derives.
+  apply derives_refl.
+  intro rho; unfold SEPx.
+  rewrite fold_right_sepcon_app.
+  assumption.
++
+  apply derives_trans
+  with (TCEXPRLIST && local (tc_environ Delta) && |> PROPx P (LOCALx Q (SEPx R))).
+  { rewrite andp_comm. solve_andp. }
+  rewrite VUNDEF.
+  apply (local2ptree_soundness P _ R) in PTREE.
+  simpl app in PTREE.
+  apply msubst_eval_exprlist_eq with (P0:=P)(R0:=R)(GV0:=GV) in MSUBST.
+  rewrite PTREE.
+  apply later_left2.
+  normalize. clear VUNDEF; rename H into VUNDEF. rewrite andp_assoc. apply andp_left2.
+  apply derives_trans with (local ((` (eq vl)) (eval_exprlist (argtypes argsig) bl)) && PROPx P (LOCALx (LocalD Qtemp Qvar GV) (SEPx R))); [rewrite (add_andp _ _ MSUBST); solve_andp |].
+  clear MSUBST.
+  intro rho.
+  apply (local2ptree_soundness nil _ (TT::nil)) in PTREE'.
+  simpl app in PTREE'.
+  rewrite !isolate_LOCAL_lem1 in PTREE'.
+  unfold local at 1, lift1.
+  simpl.
+  apply derives_extract_prop; intro. unfold_lift in H. subst vl.
+  unfold PROPx, LOCALx, SEPx. simpl.
+  apply andp_left2. apply andp_left1.
+  assert (LEN': length (var_names argsig) = length (eval_exprlist (argtypes argsig) bl rho)).
+  clear - LEN.
+  revert bl LEN; induction argsig as [ | [? ?]]; destruct bl;
+    simpl; intros; auto.
+  inv LEN.
+  forget (argtypes argsig) as tys.
+  cut (local (fold_right `(and) `(True) (map locald_denote (LocalD Qtemp Qvar GV))) rho |--
+             `(local (fold_right `(and) `(True) (map locald_denote Qpre)))
+             (fun rho => (make_args (var_names argsig) (eval_exprlist tys bl rho) rho)) rho).
+  intro. eapply derives_trans; [apply H  |].
+  unfold make_args'. simpl @fst. change (map fst argsig) with (var_names argsig).
+  clear.  unfold_lift. unfold local, lift1. apply prop_derives.
+  induction Qpre; simpl; auto.  intros [? ?]. split; auto.
+  rewrite PTREE'. clear PTREE' Qpre.
+  apply prop_derives; intro. forget (var_names argsig) as fl.
+  forget (eval_exprlist tys bl rho) as vl.
+  eapply check_specs_lemma; try eassumption.
+Qed.
+*)
 
 Lemma tc_exprlist_len : forall {cs : compspecs} Delta argsig bl,
   tc_exprlist Delta (argtypes argsig) bl |-- !!(length (argtypes argsig) = length bl).
@@ -1570,9 +1765,87 @@ eapply semax_pre_post' ; [ | |
 *
 assumption.
 Qed.
-        *)
+ *)
 
 Lemma semax_call_id00_wow:
+ forall  
+  (cs: compspecs) Qtemp Qvar a GV Delta P Q R R'
+   fs argsig retty cc ts (A: rmaps.TypeTree)  Pre Post NEPre NEPost
+   (witness: functors.MixVariantFunctor._functor (rmaps.dependent_type_functor_rec ts A) mpred) 
+   (Frame: list mpred)
+   (bl: list expr)
+   (Ppre: list Prop) (Qpre : list localdef) (Rpre: list mpred)
+   (Qactuals Qpre_temp : PTree.t _) GV'
+   (vl : list val)
+   (SETUP: call_setup2 cs Qtemp Qvar GV a Delta P Q R R' fs argsig retty cc ts A Pre Post NEPre NEPost bl vl Qactuals
+      witness Frame Ppre Qpre Rpre Qpre_temp GV')
+  Espec 
+             (Post2: environ -> mpred)
+             (B: Type)
+             (Ppost: B -> list Prop)
+             (Rpost: B -> list mpred)
+   (RETTY: retty = Tvoid)
+   (POST1: Post ts witness = (EX vret:B, PROPx (Ppost vret) (LOCALx nil (SEPx (Rpost vret)))))
+   (POST2: Post2 = EX vret:B, PROPx (P++ Ppost vret ) (LOCALx Q
+             (SEPx (Rpost vret ++ Frame))))
+   (PPRE: fold_right_and True Ppre),
+   @semax cs Espec Delta (PROPx P (LOCALx Q (SEPx R')))
+    (Scall None a bl)
+    (normal_ret_assert Post2).
+Proof.
+intros.
+destruct SETUP as [[PTREE [Hsub [SPEC (*[HR'*) [ATY [TC0 [TC1 [MSUBST PTREE'']]]]]]](*]*)
+                            [HR' [PRE1 [PTREE' [CHECKTEMP [CHECKG FRAME]]]]]].
+apply SPEC. clear SPEC.
+apply semax_pre
+with  ((tc_expr Delta a && tc_exprlist Delta (argtypes argsig) bl) &&
+       ((EX v : val, lift0 (func_ptr fs v) && local ((` (eq v)) (eval_expr a)))%assert &&
+       (!!(Datatypes.length (argtypes argsig) = Datatypes.length bl) &&
+         !!(Forall (check_one_temp_spec Qactuals) (PTree.elements Qpre_temp)) &&
+        PROPx P (LOCALx Q (SEPx R'))))).
+(*[apply andp_right; [apply andp_left2, andp_left1, derives_refl|]|].*)
+{ apply andp_right; [| apply andp_right; [apply andp_left2, andp_left1, derives_refl|]].
+  eapply derives_trans; [| apply andp_right; [ apply TC0 | apply TC1]].
+  apply andp_derives; [ | apply andp_left2]; trivial.
+  rewrite <- andp_assoc, andp_comm.
+  rewrite <- andp_assoc; apply andp_left1. apply andp_right. 2: solve_andp.
+  (*eapply derives_trans; [ | apply now_later].*)
+  rewrite andp_comm.
+  apply andp_right; trivial. 
+  eapply derives_trans; [ apply TC1 | apply tc_exprlist_len]. }
+(*rewrite later_andp.*)
+rewrite andp_comm, andp_assoc. rewrite <- andp_comm. (* rewrite <- andp_assoc.*)
+remember (tc_expr Delta a && tc_exprlist Delta (argtypes argsig) bl) as TChecks.
+rewrite ! andp_assoc. 
+apply semax_extract_prop; intros. 
+apply semax_extract_prop; intros. 
+(*rewrite <- !prop_and. rewrite ! andp_assoc.*)
+(*apply semax_extract_later_prop; intros [].*)
+rewrite andp_comm.
+eapply semax_pre_post'; [ | |
+   apply (@semax_call0 Espec cs Delta fs A Pre Post NEPre NEPost 
+              ts witness argsig retty cc a bl P Q Frame Hsub)].
+*
+  subst TChecks. eapply semax_call_aux55; eauto.
+*
+ subst.
+ clear CHECKTEMP TC1 PRE1 PPRE.
+ intros. normalize.
+ rewrite POST1; clear POST1.
+ unfold ifvoid.
+ go_lowerx. normalize.
+ apply exp_right with x.
+ rewrite fold_right_and_app_low.
+ rewrite fold_right_sepcon_app.
+ apply andp_right.
+ apply prop_right.
+ split; auto.
+ normalize.
+*
+assumption.
+Qed.
+
+Lemma semax_call_id00_wow_nil:
  forall  
   (cs: compspecs) Qtemp Qvar GV a Delta P Q R R'
    fs argsig retty cc (A: rmaps.TypeTree)  Pre Post NEPre NEPost
@@ -1582,7 +1855,7 @@ Lemma semax_call_id00_wow:
    (Ppre: list Prop) (Qpre : list localdef) (Rpre: list mpred)
    (Qactuals Qpre_temp : PTree.t _) GV'
    (vl : list val)
-   (SETUP: call_setup2 cs Qtemp Qvar GV a Delta P Q R R' fs argsig retty cc A Pre Post NEPre NEPost bl vl Qactuals
+   (SETUP: call_setup2_nil cs Qtemp Qvar GV a Delta P Q R R' fs argsig retty cc A Pre Post NEPre NEPost bl vl Qactuals
       witness Frame Ppre Qpre Rpre Qpre_temp GV')
   Espec 
              (Post2: environ -> mpred)
@@ -1598,7 +1871,8 @@ Lemma semax_call_id00_wow:
     (Scall None a bl)
     (normal_ret_assert Post2).
 Proof.
-intros.
+  intros. rewrite call_setup2_nil_equiv in SETUP.  eapply semax_call_id00_wow; eassumption.  Qed.
+(*OLD PROOF
 destruct SETUP as [[PTREE [Hsub [SPEC (*[HR'*) [ATY [TC0 [TC1 [MSUBST PTREE'']]]]]]](*]*)
                             [HR' [PRE1 [PTREE' [CHECKTEMP [CHECKG FRAME]]]]]].
 apply SPEC. clear SPEC.
@@ -1649,7 +1923,8 @@ eapply semax_pre_post'; [ | |
 *
 assumption.
 Qed.
-
+ *)
+(*
 Lemma OLDsemax_call_id1_wow:
  forall  
   (cs: compspecs) Qtemp Qvar GV a Delta P Q R R'
@@ -1730,8 +2005,102 @@ Abort. (*eapply OLDsemax_call_aux55; eauto.
  rewrite !fold_right_and_app_low in H4. destruct H4; split; auto.
 Abort.
 *)
+*)
 
 Lemma semax_call_id1_wow:
+ forall  
+  (cs: compspecs) Qtemp Qvar GV a Delta P Q R R'
+   fs argsig retty cc ts (A: rmaps.TypeTree)  Pre Post NEPre NEPost
+   (witness: functors.MixVariantFunctor._functor (rmaps.dependent_type_functor_rec ts A) mpred) 
+   (Frame: list mpred)
+   (bl: list expr)
+   (Ppre: list Prop) (Qpre : list localdef) (Rpre: list mpred)
+   (Qactuals Qpre_temp : PTree.t _) GV'
+   (vl : list val)
+   (SETUP: call_setup2 cs Qtemp Qvar GV a Delta P Q R R' fs argsig retty cc ts A Pre Post NEPre NEPost bl vl Qactuals
+      witness Frame Ppre Qpre Rpre Qpre_temp GV')
+   ret (Post2: environ -> mpred)  (Qnew: list localdef)
+    (B: Type) (Ppost: B -> list Prop) (F: B -> val) (Rpost: B -> list mpred) Espec
+   (TYret: typeof_temp Delta ret = Some retty)
+   (OKretty: check_retty retty)
+   (POST1: Post ts witness = EX vret:B, PROPx (Ppost vret)
+                              (LOCALx (temp ret_temp (F vret) :: nil)
+                              (SEPx (Rpost vret))))
+   (DELETE: remove_localdef_temp ret Q = Qnew)
+   (H0: Post2 = EX vret:B, PROPx (P++ Ppost vret) (LOCALx (temp ret (F vret) :: Qnew)
+             (SEPx (Rpost vret ++ Frame))))
+   (PPRE: fold_right_and True Ppre),
+   @semax cs Espec Delta (PROPx P (LOCALx Q (SEPx R')))
+    (Scall (Some ret) a bl)
+    (normal_ret_assert Post2).
+Proof.
+intros. 
+destruct SETUP as [[PTREE [Hsub [SPEC (*[HR'*) [ATY [TC0 [TC1 [MSUBST PTREE'']]]]]]](*]*)
+                            [HR' [PRE1 [PTREE' [CHECKTEMP [CHECKG FRAME]]]]]].
+apply SPEC. clear SPEC.
+apply semax_pre
+with  ((tc_expr Delta a && tc_exprlist Delta (argtypes argsig) bl) &&
+       ((EX v : val, lift0 (func_ptr fs v) && local ((` (eq v)) (eval_expr a)))%assert &&
+       (!!(Datatypes.length (argtypes argsig) = Datatypes.length bl) &&
+         !!(Forall (check_one_temp_spec Qactuals) (PTree.elements Qpre_temp)) &&
+        PROPx P (LOCALx Q (SEPx R'))))).
+(*[apply andp_right; [apply andp_left2, andp_left1, derives_refl|]|].*)
+{ apply andp_right; [| apply andp_right; [apply andp_left2, andp_left1, derives_refl|]].
+  eapply derives_trans; [| apply andp_right; [ apply TC0 | apply TC1]].
+  apply andp_derives; [ | apply andp_left2]; trivial.
+  rewrite <- andp_assoc, andp_comm.
+  rewrite <- andp_assoc; apply andp_left1. apply andp_right. 2: solve_andp.
+  (*eapply derives_trans; [ | apply now_later].*)
+  rewrite andp_comm.
+  apply andp_right; trivial. 
+  eapply derives_trans; [ apply TC1 | apply tc_exprlist_len]. }
+(*rewrite later_andp.*)
+rewrite andp_comm, andp_assoc. rewrite <- andp_comm. (* rewrite <- andp_assoc.*)
+remember (tc_expr Delta a && tc_exprlist Delta (argtypes argsig) bl) as TChecks.
+rewrite ! andp_assoc. 
+apply semax_extract_prop; intros. 
+apply semax_extract_prop; intros. 
+(*rewrite <- !prop_and. rewrite ! andp_assoc.*)
+(*apply semax_extract_later_prop; intros [].*)
+rewrite andp_comm.
+
+eapply semax_pre_post'; [ | |
+   apply (@semax_call1 Espec cs Delta fs A Pre Post NEPre NEPost 
+              ts witness ret argsig retty cc a bl P Q Frame Hsub)];
+ [ | 
+ | assumption
+ | clear - OKretty; destruct retty; inv OKretty; apply I
+ | hnf; clear - TYret; unfold typeof_temp in TYret;
+      destruct ((temp_types Delta) ! ret); inv TYret; auto
+ ].
+*
+subst TChecks; eapply semax_call_aux55; eauto.
+*
+ subst.
+ clear CHECKTEMP TC1 PRE1 PPRE.
+ intros.
+ normalize.
+ rewrite POST1; clear POST1.
+ apply derives_trans with
+   (EX  vret : B,
+    `(PROPx (Ppost vret)
+     (LOCAL  (temp ret_temp (F vret))
+      (SEPx (Rpost vret))))%assert (get_result1 ret)
+     * (local (tc_environ Delta) && PROPx P (LOCALx (remove_localdef_temp ret Q) (SEPx Frame)))).
+ clear.
+ go_lowerx. normalize. apply exp_right with x; normalize.
+ apply exp_left; intro vret. apply exp_right with vret.
+ normalize.
+ progress (autorewrite with norm1 norm2); normalize.
+ rewrite PROP_combine.
+ unfold fold_right.
+ go_lowerx.
+ repeat apply andp_right; try apply prop_right; auto.
+ rewrite !fold_right_and_app_low.
+ rewrite !fold_right_and_app_low in H4. destruct H4; split; auto.
+Qed.
+
+Lemma semax_call_id1_wow_nil:
  forall  
   (cs: compspecs) Qtemp Qvar GV a Delta P Q R R'
    fs argsig retty cc (A: rmaps.TypeTree)  Pre Post NEPre NEPost
@@ -1741,7 +2110,7 @@ Lemma semax_call_id1_wow:
    (Ppre: list Prop) (Qpre : list localdef) (Rpre: list mpred)
    (Qactuals Qpre_temp : PTree.t _) GV'
    (vl : list val)
-   (SETUP: call_setup2 cs Qtemp Qvar GV a Delta P Q R R' fs argsig retty cc A Pre Post NEPre NEPost bl vl Qactuals
+   (SETUP: call_setup2_nil cs Qtemp Qvar GV a Delta P Q R R' fs argsig retty cc A Pre Post NEPre NEPost bl vl Qactuals
       witness Frame Ppre Qpre Rpre Qpre_temp GV')
    ret (Post2: environ -> mpred)  (Qnew: list localdef)
     (B: Type) (Ppost: B -> list Prop) (F: B -> val) (Rpost: B -> list mpred) Espec
@@ -1758,7 +2127,8 @@ Lemma semax_call_id1_wow:
     (Scall (Some ret) a bl)
     (normal_ret_assert Post2).
 Proof.
-intros. 
+  intros. rewrite call_setup2_nil_equiv in SETUP. eapply semax_call_id1_wow; eassumption. Qed.
+(*OLD PROOF 
 destruct SETUP as [[PTREE [Hsub [SPEC (*[HR'*) [ATY [TC0 [TC1 [MSUBST PTREE'']]]]]]](*]*)
                             [HR' [PRE1 [PTREE' [CHECKTEMP [CHECKG FRAME]]]]]].
 apply SPEC. clear SPEC.
@@ -1823,6 +2193,7 @@ subst TChecks; eapply semax_call_aux55; eauto.
  rewrite !fold_right_and_app_low.
  rewrite !fold_right_and_app_low in H4. destruct H4; split; auto.
 Qed.
+ *)
 (*
 Lemma OLDsemax_call_id1_x_wow:
  forall  (cs: compspecs) Qtemp Qvar GV a Delta P Q R R'
@@ -1923,16 +2294,17 @@ Proof.
     rewrite H7 in H0 by auto; clear H7.
     split; congruence.
 Qed.*)
+
 Lemma semax_call_id1_x_wow:
  forall  (cs: compspecs) Qtemp Qvar GV a Delta P Q R R'
-   fs argsig retty' cc (A: rmaps.TypeTree)  Pre Post NEPre NEPost
-   (witness: functors.MixVariantFunctor._functor (rmaps.dependent_type_functor_rec nil A) mpred) 
+   fs argsig retty' cc ts (A: rmaps.TypeTree)  Pre Post NEPre NEPost
+   (witness: functors.MixVariantFunctor._functor (rmaps.dependent_type_functor_rec ts A) mpred) 
    (Frame: list mpred)
    (bl: list expr)
    (Ppre: list Prop) (Qpre : list localdef) (Rpre: list mpred)
    (Qactuals Qpre_temp : PTree.t _) GV'
    (vl : list val)
-   (SETUP: call_setup2 cs Qtemp Qvar GV a Delta P Q R R' fs argsig retty' cc A Pre Post NEPre NEPost bl vl Qactuals
+   (SETUP: call_setup2 cs Qtemp Qvar GV a Delta P Q R R' fs argsig retty' cc ts A Pre Post NEPre NEPost bl vl Qactuals
       witness Frame Ppre Qpre Rpre Qpre_temp GV')
    retty  Espec ret ret'
              (Post2: environ -> mpred)
@@ -1947,7 +2319,7 @@ Lemma semax_call_id1_x_wow:
    (OKretty': check_retty retty')
    (NEUTRAL: is_neutral_cast retty' retty = true)
    (NEret: ret <> ret')
-   (POST1: Post nil witness = EX vret:B, PROPx (Ppost vret)
+   (POST1: Post ts witness = EX vret:B, PROPx (Ppost vret)
                               (LOCALx (temp ret_temp (F vret) :: nil)
                               (SEPx (Rpost vret))))
    (DELETE: remove_localdef_temp ret Q = Qnew)
@@ -2022,6 +2394,108 @@ Proof.
     rewrite H7 in H0 by auto; clear H7.
     split; congruence.
 Qed.
+
+Lemma semax_call_id1_x_wow_nil:
+ forall  (cs: compspecs) Qtemp Qvar GV a Delta P Q R R'
+   fs argsig retty' cc (A: rmaps.TypeTree)  Pre Post NEPre NEPost
+   (witness: functors.MixVariantFunctor._functor (rmaps.dependent_type_functor_rec nil A) mpred) 
+   (Frame: list mpred)
+   (bl: list expr)
+   (Ppre: list Prop) (Qpre : list localdef) (Rpre: list mpred)
+   (Qactuals Qpre_temp : PTree.t _) GV'
+   (vl : list val)
+   (SETUP: call_setup2_nil cs Qtemp Qvar GV a Delta P Q R R' fs argsig retty' cc A Pre Post NEPre NEPost bl vl Qactuals
+      witness Frame Ppre Qpre Rpre Qpre_temp GV')
+   retty  Espec ret ret'
+             (Post2: environ -> mpred)
+             (Qnew: list localdef)
+             (B: Type)
+             (Ppost: B -> list Prop)
+             (F: B -> val)
+             (Rpost: B -> list mpred)
+   (TYret: typeof_temp Delta ret = Some retty)
+   (RETinit: (temp_types Delta) ! ret' = Some retty')
+   (OKretty: check_retty retty)
+   (OKretty': check_retty retty')
+   (NEUTRAL: is_neutral_cast retty' retty = true)
+   (NEret: ret <> ret')
+   (POST1: Post nil witness = EX vret:B, PROPx (Ppost vret)
+                              (LOCALx (temp ret_temp (F vret) :: nil)
+                              (SEPx (Rpost vret))))
+   (DELETE: remove_localdef_temp ret Q = Qnew)
+   (DELETE' : remove_localdef_temp ret' Q = Q)
+   (H0: Post2 = EX vret:B, PROPx (P++ Ppost vret)
+                   (LOCALx (temp ret (F vret) :: Qnew)
+                    (SEPx (Rpost vret ++ Frame))))
+   (PPRE: fold_right_and True Ppre),
+   @semax cs Espec Delta (PROPx P (LOCALx Q (SEPx R')))
+   (Ssequence (Scall (Some ret') a bl)
+      (Sset ret (Ecast (Etempvar ret' retty') retty)))
+    (normal_ret_assert Post2).
+Proof.
+  intros. rewrite call_setup2_nil_equiv in SETUP. eapply semax_call_id1_x_wow; eassumption. Qed.
+(*OLD PROOF 
+  eapply semax_seq'.
+  eapply semax_call_id1_wow; try eassumption; auto.
+  unfold typeof_temp; rewrite RETinit; reflexivity.
+  apply extract_exists_pre; intro vret.
+  eapply semax_pre_post';
+    [ | | apply semax_set_forward].
+  + eapply derives_trans; [ | apply now_later ].
+    instantiate (1:= (PROPx (P ++ Ppost vret)
+      (LOCALx (temp ret' (F vret) :: Qnew) (SEPx (Rpost vret ++ Frame))))).
+    apply andp_right; [apply andp_right |].
+    - unfold tc_expr.
+      simpl typecheck_expr.
+      rewrite RETinit.
+      simpl @fst.
+      replace ((is_neutral_cast retty' retty' || same_base_type retty' retty')%bool)
+        with true
+        by (clear- OKretty'; destruct retty' as [ | [ | | |] [| ]| [|] | [ | ] |  | | | | ]; try contradiction; unfold is_neutral_cast; rewrite ?eqb_type_refl; reflexivity).
+      rewrite denote_tc_assert_andp.
+      apply andp_right; [| intros rho; apply neutral_isCastResultType; auto].
+      apply PQR_denote_tc_initialized; auto.
+    - unfold tc_temp_id, typecheck_temp_id.
+      unfold typeof_temp in TYret.
+      destruct ((temp_types Delta) ! ret); inversion TYret; clear TYret; try subst t.
+      go_lowerx.
+      repeat rewrite denote_tc_assert_andp; simpl.
+      rewrite denote_tc_assert_bool.
+      assert (is_neutral_cast (implicit_deref retty) retty = true).
+      {
+        destruct retty as [ | [ | | |] [| ]| [|] | [ | ] |  | | | | ]; try contradiction; try reflexivity;
+        destruct retty' as [ | [ | | |] [| ]| [|] | [ | ] |  | | | | ]; try contradiction; 
+        try solve [inv NEUTRAL].
+        unfold implicit_deref, is_neutral_cast. rewrite eqb_type_refl; reflexivity.
+      }
+      simpl; apply andp_right. apply prop_right; auto.
+      apply neutral_isCastResultType; auto.
+    - rewrite <- !insert_local. apply andp_left2.
+      apply andp_derives; auto.
+      subst Qnew; apply derives_remove_localdef_PQR.
+  + intros. subst Post2.
+    normalize.
+    apply exp_right with vret; normalize.
+    rewrite <- !insert_local.
+    autorewrite with subst.
+    rewrite <- !andp_assoc.
+    apply andp_derives; [| subst Qnew; apply subst_remove_localdef_PQR].
+    go_lowerx.
+    unfold_lift.
+    normalize.
+    assert (eqb_ident ret ret' = false)
+    by (clear - NEret; pose proof (eqb_ident_spec ret ret');
+        destruct (eqb_ident ret ret'); auto;
+        contradiction NEret; intuition).
+    rewrite H3 in *. apply Pos.eqb_neq in H3.
+    unfold_lift in H0.
+    assert (tc_val retty' (eval_id ret' rho))
+      by (eapply tc_eval'_id_i; try eassumption; congruence).
+    assert (H7 := expr2.neutral_cast_lemma); unfold eval_cast in H7.
+    rewrite H7 in H0 by auto; clear H7.
+    split; congruence.
+Qed.
+ *)
 (*
 Lemma OLDsemax_call_id1_y_wow:
  forall  (cs: compspecs) Qtemp Qvar GV a Delta P Q R R'
@@ -2118,14 +2592,14 @@ Proof.
 Qed.*)
 Lemma semax_call_id1_y_wow:
  forall  (cs: compspecs) Qtemp Qvar GV a Delta P Q R R'
-   fs argsig retty' cc (A: rmaps.TypeTree)  Pre Post NEPre NEPost
-   (witness: functors.MixVariantFunctor._functor (rmaps.dependent_type_functor_rec nil A) mpred) 
+   fs argsig retty' cc ts (A: rmaps.TypeTree)  Pre Post NEPre NEPost
+   (witness: functors.MixVariantFunctor._functor (rmaps.dependent_type_functor_rec ts A) mpred) 
    (Frame: list mpred)
    (bl: list expr)
    (Ppre: list Prop) (Qpre : list localdef) (Rpre: list mpred)
    (Qactuals Qpre_temp : PTree.t _) GV'
    (vl : list val)
-   (SETUP: call_setup2 cs Qtemp Qvar GV a Delta P Q R R' fs argsig retty' cc A Pre Post NEPre NEPost bl vl Qactuals
+   (SETUP: call_setup2 cs Qtemp Qvar GV a Delta P Q R R' fs argsig retty' cc ts A Pre Post NEPre NEPost bl vl Qactuals
       witness Frame Ppre Qpre Rpre Qpre_temp GV')
     Espec ret ret' (retty: type) 
              (Post2: environ -> mpred)
@@ -2140,7 +2614,7 @@ Lemma semax_call_id1_y_wow:
    (OKretty': check_retty retty')
    (NEUTRAL: is_neutral_cast retty' retty = true)
    (NEret: ret <> ret')
-   (POST1: Post nil witness = EX vret:B, PROPx (Ppost vret)
+   (POST1: Post ts witness = EX vret:B, PROPx (Ppost vret)
                               (LOCALx (temp ret_temp (F vret) :: nil)
                               (SEPx (Rpost vret))))
    (DELETE: remove_localdef_temp ret Q = Qnew)
@@ -2208,6 +2682,186 @@ Proof.
         contradiction NEret; intuition).
     rewrite H3 in *. apply Pos.eqb_neq in H3.
     split; congruence.
+Qed.
+
+Lemma semax_call_id1_y_wow_nil:
+ forall  (cs: compspecs) Qtemp Qvar GV a Delta P Q R R'
+   fs argsig retty' cc (A: rmaps.TypeTree)  Pre Post NEPre NEPost
+   (witness: functors.MixVariantFunctor._functor (rmaps.dependent_type_functor_rec nil A) mpred) 
+   (Frame: list mpred)
+   (bl: list expr)
+   (Ppre: list Prop) (Qpre : list localdef) (Rpre: list mpred)
+   (Qactuals Qpre_temp : PTree.t _) GV'
+   (vl : list val)
+   (SETUP: call_setup2_nil cs Qtemp Qvar GV a Delta P Q R R' fs argsig retty' cc A Pre Post NEPre NEPost bl vl Qactuals
+      witness Frame Ppre Qpre Rpre Qpre_temp GV')
+    Espec ret ret' (retty: type) 
+             (Post2: environ -> mpred)
+             (Qnew: list localdef)
+             (B: Type)
+             (Ppost: B -> list Prop)
+             (F: B -> val)
+             (Rpost: B -> list mpred)
+   (TYret: typeof_temp Delta ret = Some retty)
+   (RETinit: (temp_types Delta) ! ret' = Some retty')
+   (OKretty: check_retty retty)
+   (OKretty': check_retty retty')
+   (NEUTRAL: is_neutral_cast retty' retty = true)
+   (NEret: ret <> ret')
+   (POST1: Post nil witness = EX vret:B, PROPx (Ppost vret)
+                              (LOCALx (temp ret_temp (F vret) :: nil)
+                              (SEPx (Rpost vret))))
+   (DELETE: remove_localdef_temp ret Q = Qnew)
+   (DELETE' : remove_localdef_temp ret' Q = Q)
+   (H0: Post2 = EX vret:B, PROPx (P++ Ppost vret)
+                   (LOCALx (temp ret (F vret) :: Qnew)
+                    (SEPx (Rpost vret ++ Frame))))
+   (PPRE: fold_right_and True Ppre),
+   @semax cs Espec Delta (PROPx P (LOCALx Q (SEPx R')))
+   (Ssequence (Scall (Some ret') a bl)
+      (Sset ret (Etempvar ret' retty')))
+    (normal_ret_assert Post2).
+Proof.
+  intros. rewrite call_setup2_nil_equiv in SETUP. eapply semax_call_id1_y_wow; eassumption. Qed.
+(*OLD PROOF
+  eapply semax_seq'.
+  eapply semax_call_id1_wow; try eassumption; auto;
+    unfold typeof_temp; rewrite RETinit; reflexivity.
+  apply extract_exists_pre; intro vret.
+  eapply semax_pre_post';
+    [ | | apply semax_set_forward].
+  + eapply derives_trans; [ | apply now_later ].
+    instantiate (1:= (PROPx (P ++ Ppost vret)
+      (LOCALx (temp ret' (F vret) :: Qnew) (SEPx (Rpost vret ++ Frame))))).
+    apply andp_right; [apply andp_right |].
+    - unfold tc_expr.
+      match goal with |- _ |-- ?A =>
+        set (aa:=A); unfold denote_tc_assert in aa; simpl in aa; subst aa
+      end.
+      rewrite RETinit.
+      simpl @fst.
+      replace ((is_neutral_cast retty' retty' || same_base_type retty' retty')%bool)
+        with true
+        by (clear- OKretty'; destruct retty' as [ | [ | | |] [| ]| [|] | [ | ] |  | | | | ]; try contradiction; unfold is_neutral_cast; rewrite ?eqb_type_refl; reflexivity).
+      simpl @snd. cbv iota.
+      apply PQR_denote_tc_initialized; auto.
+    - unfold tc_temp_id, typecheck_temp_id.
+      unfold typeof_temp in TYret.
+      destruct ((temp_types Delta) ! ret); inversion TYret; clear TYret; try subst t.
+      go_lowerx.
+      repeat rewrite denote_tc_assert_andp; simpl.
+      rewrite denote_tc_assert_bool.
+      assert (is_neutral_cast (implicit_deref retty') retty = true).
+      * replace (implicit_deref retty') with retty'
+          by (destruct retty' as [ | [ | | |] [| ]| [|] | [ | ] |  | | | | ]; try contradiction; reflexivity).
+        auto.
+      * simpl; apply andp_right. apply prop_right; auto.
+        apply neutral_isCastResultType; auto.
+    - rewrite <- !insert_local. apply andp_left2.
+      apply andp_derives; auto.
+      subst Qnew; apply derives_remove_localdef_PQR.
+  + intros. subst Post2.
+    unfold normal_ret_assert.
+    normalize.
+    apply exp_right with vret; normalize.
+    rewrite <- !insert_local.
+    autorewrite with subst.
+    rewrite <- !andp_assoc.
+    apply andp_derives; [| subst Qnew; apply subst_remove_localdef_PQR].
+    go_lowerx.
+    unfold_lift.
+    normalize.
+    assert (eqb_ident ret ret' = false)
+    by (clear - NEret; pose proof (eqb_ident_spec ret ret');
+        destruct (eqb_ident ret ret'); auto;
+        contradiction NEret; intuition).
+    rewrite H3 in *. apply Pos.eqb_neq in H3.
+    split; congruence.
+Qed.
+ *)
+Lemma semax_call_id01_wow:
+ forall  
+  (cs: compspecs) Qtemp Qvar GV a Delta P Q R R'
+   fs argsig retty cc ts (A: rmaps.TypeTree)  Pre Post NEPre NEPost
+   (witness: functors.MixVariantFunctor._functor (rmaps.dependent_type_functor_rec ts A) mpred) 
+   (Frame: list mpred)
+   (bl: list expr)
+   (Ppre: list Prop) (Qpre : list localdef) (Rpre: list mpred)
+   (Qactuals Qpre_temp : PTree.t _) GV'
+   (vl : list val)
+   (SETUP: call_setup2 cs Qtemp Qvar GV a Delta P Q R R' fs argsig retty cc ts A Pre Post NEPre NEPost bl vl Qactuals
+      witness Frame Ppre Qpre Rpre Qpre_temp GV')
+   Espec
+             (Post2: environ -> mpred)
+             (B: Type)
+             (Ppost: B -> list Prop)
+             (F: B -> val)
+             (Rpost: B -> list mpred)
+   (_: check_retty retty)
+         (* this hypothesis is not needed for soundness, just for selectivity *)
+   (POST1: Post ts witness = EX vret:B, PROPx (Ppost vret)
+                              (LOCALx (temp ret_temp (F vret) :: nil)
+                              (SEPx (Rpost vret))))
+   (POST2: Post2 = EX vret:B, PROPx (P++ Ppost vret) (LOCALx Q
+             (SEPx (Rpost vret ++ Frame))))
+   (PPRE: fold_right_and True Ppre),
+   @semax cs Espec Delta (PROPx P (LOCALx Q (SEPx R')))
+    (Scall None a bl)
+    (normal_ret_assert Post2).
+Proof.
+intros.
+destruct SETUP as [[PTREE [Hsub [SPEC (*[HR'*) [ATY [TC0 [TC1 [MSUBST PTREE'']]]]]]](*]*)
+                            [HR' [PRE1 [PTREE' [CHECKTEMP [CHECKG FRAME]]]]]].
+apply SPEC. clear SPEC.
+apply semax_pre
+with  ((tc_expr Delta a && tc_exprlist Delta (argtypes argsig) bl) &&
+       ((EX v : val, lift0 (func_ptr fs v) && local ((` (eq v)) (eval_expr a)))%assert &&
+       (!!(Datatypes.length (argtypes argsig) = Datatypes.length bl) &&
+         !!(Forall (check_one_temp_spec Qactuals) (PTree.elements Qpre_temp)) &&
+        PROPx P (LOCALx Q (SEPx R'))))).
+(*[apply andp_right; [apply andp_left2, andp_left1, derives_refl|]|].*)
+{ apply andp_right; [| apply andp_right; [apply andp_left2, andp_left1, derives_refl|]].
+  eapply derives_trans; [| apply andp_right; [ apply TC0 | apply TC1]].
+  apply andp_derives; [ | apply andp_left2]; trivial.
+  rewrite <- andp_assoc, andp_comm.
+  rewrite <- andp_assoc; apply andp_left1. apply andp_right. 2: solve_andp.
+  (*eapply derives_trans; [ | apply now_later].*)
+  rewrite andp_comm.
+  apply andp_right; trivial. 
+  eapply derives_trans; [ apply TC1 | apply tc_exprlist_len]. }
+(*rewrite later_andp.*)
+rewrite andp_comm, andp_assoc. rewrite <- andp_comm. (* rewrite <- andp_assoc.*)
+remember (tc_expr Delta a && tc_exprlist Delta (argtypes argsig) bl) as TChecks.
+rewrite ! andp_assoc. 
+apply semax_extract_prop; intros. 
+apply semax_extract_prop; intros. 
+(*rewrite <- !prop_and. rewrite ! andp_assoc.*)
+(*apply semax_extract_later_prop; intros [].*)
+rewrite andp_comm.
+
+eapply semax_pre_post';
+   [ |
+   | apply semax_call0 with (fs:=fs)(cc:=cc)(A:= A) (ts := ts)(x:=witness) (P:=P)(Q:=Q)(NEPre :=NEPre) (NEPost := NEPost)(R := Frame)
+   ];
+   try eassumption.
+* subst TChecks. eapply semax_call_aux55; eauto.
+*
+ subst.
+ clear CHECKTEMP TC1 PRE1 PPRE.
+ intros.
+ normalize.
+ rewrite POST1; clear POST1.
+ match goal with |- context [ifvoid retty ?A ?B] =>
+   replace (ifvoid retty A B) with B
+   by (destruct retty; try contradiction; auto)
+ end.
+ go_lowerx. normalize. apply exp_right with x0; normalize.
+ apply andp_right; auto.
+ apply prop_right.
+ rewrite fold_right_and_app_low. split; auto.
+ rename x0 into vret.
+ clear.
+ rewrite fold_right_sepcon_app. auto.
 Qed.
 
 (*
@@ -2282,7 +2936,8 @@ eapply semax_pre_post';
  clear.
  rewrite fold_right_sepcon_app. auto.
 Qed.*)
-Lemma semax_call_id01_wow:
+
+Lemma semax_call_id01_wow_nil:
  forall  
   (cs: compspecs) Qtemp Qvar GV a Delta P Q R R'
    fs argsig retty cc (A: rmaps.TypeTree)  Pre Post NEPre NEPost
@@ -2292,7 +2947,7 @@ Lemma semax_call_id01_wow:
    (Ppre: list Prop) (Qpre : list localdef) (Rpre: list mpred)
    (Qactuals Qpre_temp : PTree.t _) GV'
    (vl : list val)
-   (SETUP: call_setup2 cs Qtemp Qvar GV a Delta P Q R R' fs argsig retty cc A Pre Post NEPre NEPost bl vl Qactuals
+   (SETUP: call_setup2_nil cs Qtemp Qvar GV a Delta P Q R R' fs argsig retty cc A Pre Post NEPre NEPost bl vl Qactuals
       witness Frame Ppre Qpre Rpre Qpre_temp GV')
    Espec
              (Post2: environ -> mpred)
@@ -2312,7 +2967,8 @@ Lemma semax_call_id01_wow:
     (Scall None a bl)
     (normal_ret_assert Post2).
 Proof.
-intros.
+intros. rewrite call_setup2_nil_equiv in SETUP. eapply semax_call_id01_wow; eassumption. Qed.
+(*OLD PROOF
 destruct SETUP as [[PTREE [Hsub [SPEC (*[HR'*) [ATY [TC0 [TC1 [MSUBST PTREE'']]]]]]](*]*)
                             [HR' [PRE1 [PTREE' [CHECKTEMP [CHECKG FRAME]]]]]].
 apply SPEC. clear SPEC.
@@ -2366,7 +3022,7 @@ eapply semax_pre_post';
  clear.
  rewrite fold_right_sepcon_app. auto.
 Qed.
-
+ *)
 
 Lemma match_funcptr'_funcptr:
  forall fs v B, 
